Syntactic Viper-Boogie relation and proof of its correctness
Integer division and modulo are currently not captured, because there is a mismatch between the Viper and Boogie formalization. We need to decide what the semantics of Div and Mod should be in Viper.

ViperBoogieBasicRel.thy
@@ -15,9 +15,9 @@ type_synonym 'a bpl_mask_ty = "ref \<Rightarrow> 'a vb_field \<Rightarrow> real"
 record tr_vpr_bpl =
   heap_var :: Lang.vname
   mask_var :: Lang.vname
-  mask_read :: "expr \<Rightarrow> expr \<Rightarrow> expr \<Rightarrow> expr" \<comment>\<open>arguments: heap, receiver, field\<close>
+  mask_read :: "expr \<Rightarrow> expr \<Rightarrow> expr \<Rightarrow> expr" \<comment>\<open>arguments: mask, receiver, field\<close>
   heap_read :: "expr \<Rightarrow> expr \<Rightarrow> expr \<Rightarrow> expr" \<comment>\<open>arguments: heap, receiver, field\<close>
-  field_translation :: "field_ident \<rightharpoonup> field_ident"
+  field_translation :: "field_ident \<rightharpoonup> Lang.vname"
   fun_translation :: "ViperLang.function_ident \<rightharpoonup> Lang.fname"
   var_translation :: "ViperLang.var \<rightharpoonup> Lang.vname" \<comment>\<open>local Boogie variables\<close>
   lit_translation :: "ViperLang.lit \<Rightarrow> expr"
@@ -37,17 +37,18 @@ fun val_rel_vpr_bpl :: "'a vpr_val \<Rightarrow> 'a vbpl_val"
 
 subsection \<open>State relationship\<close>
 
-definition heap_rel :: "ViperLang.program \<Rightarrow> (field_ident \<rightharpoonup> field_ident) \<Rightarrow> 'a total_heap \<Rightarrow> 'a bpl_heap_ty \<Rightarrow> bool"
+definition heap_rel :: "ViperLang.program \<Rightarrow> (field_ident \<rightharpoonup> vname) \<Rightarrow> 'a total_heap \<Rightarrow> 'a bpl_heap_ty \<Rightarrow> bool"
   where "heap_rel Pr tr_field h hb \<equiv> 
     \<forall> l :: heap_loc. if_Some 
-                       (\<lambda>field_vty. option_fold (\<lambda>res. val_rel_vpr_bpl (h l) = res) False (hb (Address (fst l)) (NormalField (the (tr_field (snd l))) field_vty)))
+                       (\<lambda>field_vty. has_Some (\<lambda>res. val_rel_vpr_bpl (h l) = res) (hb (Address (fst l)) (NormalField (the (tr_field (snd l))) field_vty)))
                        (declared_fields Pr (snd l))"
 
-definition mask_rel :: "ViperLang.program \<Rightarrow> (field_ident \<rightharpoonup> field_ident) \<Rightarrow> mask \<Rightarrow> 'a bpl_mask_ty \<Rightarrow> bool"
+definition mask_rel :: "ViperLang.program \<Rightarrow> (field_ident \<rightharpoonup> vname) \<Rightarrow> mask \<Rightarrow> 'a bpl_mask_ty \<Rightarrow> bool"
   where "mask_rel Pr tr_field m mb \<equiv> 
-    \<forall> l :: heap_loc. if_Some 
+    (\<forall> l :: heap_loc. if_Some 
                        (\<lambda>field_vty. real_of_rat (Rep_prat (m l)) = (mb (Address (fst l)) (NormalField (the (tr_field (snd l))) field_vty)))
-                       (declared_fields Pr (snd l))"
+                       (declared_fields Pr (snd l))) \<and>
+    (\<forall>f t. mb Null (NormalField f t) = 0)"
 
 text \<open>\<^const>\<open>heap_rel\<close> and \<^const>\<open>mask_rel\<close> depend on the program, since the Viper type of a Viper field is required (currently)
       to identify the corresponding Boogie field\<close>
@@ -60,14 +61,15 @@ definition predicate_heap_rel :: "ViperLang.program \<Rightarrow> ('a \<Rightarr
 *)
 
 (* TODO: lift to predicates *)
-definition state_rel_vpr_bpl :: "ViperLang.program \<Rightarrow> tr_vpr_bpl \<Rightarrow> 'a full_total_state \<Rightarrow> ('a vbpl_absval) nstate \<Rightarrow> bool"
-  where "state_rel_vpr_bpl Pr T \<omega> ns \<equiv>
+definition state_rel_vpr_bpl :: "ViperLang.program \<Rightarrow> var_context \<Rightarrow> tr_vpr_bpl \<Rightarrow> 'a full_total_state \<Rightarrow> ('a vbpl_absval) nstate \<Rightarrow> bool"
+  where "state_rel_vpr_bpl Pr \<Lambda> T \<omega> ns \<equiv>
            (\<forall> var_vpr var_bpl. var_translation T var_vpr = Some var_bpl \<longrightarrow> 
-              (\<exists>val_vpr val_bpl. ((get_store_total \<omega>) var_vpr) = Some val_vpr \<and>
-                                ((local_state ns) var_vpr) = Some val_bpl \<and>
-                                val_rel_vpr_bpl val_vpr = val_bpl)) \<and>
-           (\<exists>hb. (global_state ns) (heap_var T) = Some (AbsV (AHeap hb)) \<and> heap_rel Pr (field_translation T) (get_hh_total_full \<omega>) hb) \<and>
-           (\<exists>mb. (global_state ns) (mask_var T) = Some (AbsV (AMask mb)) \<and> mask_rel Pr (field_translation T) (get_mh_total_full \<omega>) mb)"
+              (\<exists>val_vpr. ((get_store_total \<omega>) var_vpr) = Some val_vpr \<and>
+                                (lookup_var \<Lambda> ns var_bpl) = Some (val_rel_vpr_bpl val_vpr))) \<and>
+           (\<exists>hb. lookup_var \<Lambda> ns (heap_var T) = Some (AbsV (AHeap hb)) \<and> heap_rel Pr (field_translation T) (get_hh_total_full \<omega>) hb) \<and>
+           (\<exists>mb. lookup_var \<Lambda> ns (mask_var T) = Some (AbsV (AMask mb)) \<and> mask_rel Pr (field_translation T) (get_mh_total_full \<omega>) mb) \<and>
+           (\<forall>f f_vty. declared_fields Pr f = Some f_vty \<longrightarrow> 
+             has_Some (\<lambda>f_bpl. lookup_var \<Lambda> ns f_bpl = Some (AbsV (AField (NormalField f_bpl f_vty)))) (field_translation T f))"
 
 subsection\<open>function relation\<close>
 
@@ -75,29 +77,36 @@ subsection\<open>function relation\<close>
 abbreviation eval_heap_dep_bpl_fun :: "('a vbpl_absval) Semantics.fun_repr \<Rightarrow> ('a vbpl_val) list \<Rightarrow> 'a vbpl_val \<rightharpoonup> 'a vbpl_val"
   where "eval_heap_dep_bpl_fun f_bpl vs heap \<equiv> f_bpl [] (heap#vs)"
 
-definition fun_rel :: "ViperLang.program \<Rightarrow> (field_ident \<rightharpoonup> field_ident) \<Rightarrow> 'a TotalExpressions.heapfun_repr \<Rightarrow> ('a vbpl_absval) Semantics.fun_repr \<Rightarrow> bool"
+definition fun_rel :: "ViperLang.program \<Rightarrow> (field_ident \<rightharpoonup> vname) \<Rightarrow> 'a TotalExpressions.heapfun_repr \<Rightarrow> ('a vbpl_absval) Semantics.fun_repr \<Rightarrow> bool"
   where "fun_rel Pr tr_field f_vpr f_bpl \<equiv> 
            (\<forall>vs \<omega> v_vpr. f_vpr vs \<omega> = Some (Val v_vpr) \<longrightarrow>
               (\<forall> h_bpl. heap_rel Pr tr_field (get_hh_total_full \<omega>) h_bpl \<longrightarrow>
                 has_Some (\<lambda>v_bpl. val_rel_vpr_bpl v_vpr = v_bpl) (eval_heap_dep_bpl_fun f_bpl ((map val_rel_vpr_bpl) vs) (AbsV (AHeap h_bpl)))))"
 
-definition fun_interp_rel :: "ViperLang.program \<Rightarrow> (field_ident \<rightharpoonup> field_ident) \<Rightarrow> (ViperLang.function_ident \<Rightarrow> Lang.fname) \<Rightarrow> 'a TotalExpressions.interp \<Rightarrow> ('a vbpl_absval) Semantics.fun_interp \<Rightarrow> bool"
+definition fun_interp_rel :: "ViperLang.program \<Rightarrow> (field_ident \<rightharpoonup> vname) \<Rightarrow> (ViperLang.function_ident \<rightharpoonup> Lang.fname) \<Rightarrow> 'a TotalExpressions.interp \<Rightarrow> ('a vbpl_absval) Semantics.fun_interp \<Rightarrow> bool"
   where 
-    "fun_interp_rel Pr tr_field f_tr \<Delta> \<Gamma> \<equiv> (\<forall>fid f_vpr. \<Delta> fid \<noteq> Some f_vpr \<longrightarrow>
-                                 has_Some (\<lambda>f_bpl. fun_rel Pr tr_field f_vpr f_bpl) (\<Gamma> (f_tr fid)))"
+    "fun_interp_rel Pr tr_field tr_fun \<Delta> \<Gamma> \<equiv> (\<forall>fid f_vpr. \<Delta> fid = Some f_vpr \<longrightarrow>
+                                 (\<forall>fid_bpl. tr_fun fid = Some fid_bpl \<longrightarrow>
+                                   has_Some (\<lambda>f_bpl. fun_rel Pr tr_field f_vpr f_bpl) (\<Gamma> fid_bpl)))"
 
 subsection \<open>expression relation\<close>
 
 record 'a context_bpl =
-  get_var_context :: var_context
-  get_fun_interp :: "('a vbpl_absval) fun_interp"
-  get_type_interp :: "('a vbpl_absval) absval_ty_fun"
+  type_interp :: "('a vbpl_absval) absval_ty_fun"
+  var_context :: var_context
+  fun_interp :: "('a vbpl_absval) fun_interp"
+
+abbreviation create_ctxt_bpl :: "('a vbpl_absval) absval_ty_fun \<Rightarrow> var_context \<Rightarrow> ('a vbpl_absval) fun_interp \<Rightarrow> 'a context_bpl"
+  where "create_ctxt_bpl A \<Lambda> \<Gamma> \<equiv> \<lparr>type_interp=A, var_context=\<Lambda>,fun_interp=\<Gamma>\<rparr>"
+
+abbreviation red_expr_bpl :: "'a context_bpl \<Rightarrow> expr \<Rightarrow> ('a vbpl_absval) nstate \<Rightarrow> 'a vbpl_val \<Rightarrow> bool"
+  where "red_expr_bpl ctxt e ns v \<equiv> type_interp ctxt,var_context ctxt, fun_interp ctxt,[] \<turnstile> \<langle>e, ns\<rangle> \<Down> v"
 
 definition exp_rel_vpr_bpl :: 
    "ViperLang.program \<Rightarrow> 'a interp \<Rightarrow> 'a ty_repr_bpl \<Rightarrow> tr_vpr_bpl \<Rightarrow> 'a context_bpl \<Rightarrow> viper_expr \<Rightarrow> boogie_expr \<Rightarrow> 'a full_total_state \<Rightarrow> ('a vbpl_absval) nstate \<Rightarrow> bool"
   where "exp_rel_vpr_bpl Pr \<Delta> T Tr ctxt e_vpr e_bpl \<omega> ns \<equiv> 
              \<exists>v1 v2. (Pr, \<Delta>, None \<turnstile> \<langle>e_vpr; \<omega>\<rangle> [\<Down>]\<^sub>t Val v1) \<and> 
-             ((get_type_interp) ctxt,(get_var_context) ctxt, (get_fun_interp) ctxt,[] \<turnstile> \<langle>e_bpl, ns\<rangle> \<Down> v2) \<and> (val_rel_vpr_bpl v1 = v2)"
+             (red_expr_bpl ctxt e_bpl ns v2) \<and> (val_rel_vpr_bpl v1 = v2)"
 
 
 subsection \<open>syntactic relations\<close>
@@ -107,12 +116,21 @@ fun unop_rel :: "ViperLang.unop \<Rightarrow> Lang.unop"
     "unop_rel ViperLang.Minus = Lang.UMinus"
   | "unop_rel ViperLang.Not = Lang.Not"
 
+lemma unop_rel_correct: 
+  assumes 
+    "eval_unop uop_vpr v_vpr = BinopNormal v_vpr'" and
+    "unop_rel uop_vpr = uop_bpl"
+  shows "unop_eval_val uop_bpl (val_rel_vpr_bpl v_vpr) = Some (val_rel_vpr_bpl v_vpr')  "
+  apply (insert assms)
+  by (erule eval_unop.elims) (auto simp: of_rat_minus)   
+
 fun binop_rel :: "ViperLang.binop \<Rightarrow> Lang.binop"
   where 
     "binop_rel ViperLang.Add = Lang.Add"
   | "binop_rel ViperLang.Sub = Lang.Sub"
   | "binop_rel ViperLang.Mult = Lang.Mul"
   | "binop_rel ViperLang.IntDiv = Lang.Div"
+  | "binop_rel ViperLang.PermDiv = Lang.RealDiv"
   | "binop_rel ViperLang.Mod = Lang.Mod"
   | "binop_rel ViperLang.Eq = Lang.Eq"
   | "binop_rel ViperLang.Neq = Lang.Neq"
@@ -123,58 +141,390 @@ fun binop_rel :: "ViperLang.binop \<Rightarrow> Lang.binop"
   | "binop_rel ViperLang.Or = Lang.Or"
   | "binop_rel ViperLang.BImp = Lang.Imp"
   | "binop_rel ViperLang.And = Lang.And"
-(* TODO: PermDiv case *)
 
+lemma binop_lazy_rel_correct:
+  assumes "eval_binop_lazy v_vpr bop_vpr = Some v'_vpr" and
+          "binop_rel bop_vpr = bop_bpl" and
+          "binop_eval_val bop_bpl (val_rel_vpr_bpl v_vpr) v_bpl \<noteq> None"
+  shows   "binop_eval_val bop_bpl (val_rel_vpr_bpl v_vpr) v_bpl = Some (val_rel_vpr_bpl v'_vpr)"
+  using assms
+  apply (cases rule: eval_binop_lazy.elims)
+  apply simp_all
+  by (cases v_bpl; (rename_tac lit, case_tac lit, auto))+
+
+lemma binop_nonlazy_rel_correct:
+  assumes "eval_binop v1_vpr bop_vpr v2_vpr = BinopNormal v_vpr" and
+          "binop_rel bop_vpr = bop_bpl" and
+           \<comment>\<open>need to update Viper semantics or change relation to deal with integer division and modulo\<close>
+          "bop_vpr \<noteq> IntDiv \<and> bop_vpr \<noteq> ViperLang.Mod" 
+  shows   "binop_eval_val bop_bpl (val_rel_vpr_bpl v1_vpr) (val_rel_vpr_bpl v2_vpr) = Some (val_rel_vpr_bpl v_vpr)"
+  using assms
+  apply (cases rule: eval_binop.elims)
+                      apply simp_all
+    apply (cases bop_vpr)
+                  apply simp_all
+     \<comment>\<open>real division of two integers\<close>
+    apply (unfold smt_real_div_def)
+    apply (metis (mono_tags, hide_lams) Fract_of_int_quotient binop_result.distinct(5) binop_result.inject of_int_0_eq_iff of_rat_divide of_rat_of_int_eq val_rel_vpr_bpl.simps(5))
+   
+   \<comment>\<open>operator betweeen two reals\<close>
+   apply (cases bop_vpr)
+                 apply (simp_all add: of_rat_add of_rat_diff of_rat_mult smt_real_div_def of_rat_less of_rat_less_eq)
+   apply (metis binop_result.distinct(5) binop_result.inject of_rat_divide val_rel_vpr_bpl.simps(5))
+
+\<comment>\<open>operator between two booleans\<close>
+  apply (cases bop_vpr) 
+                apply simp_all
+  done 
+
+  
 (*
 datatype pure_exp =
   ELit lit
   | Var var
   | Unop unop pure_exp
   | Binop pure_exp binop pure_exp
-  | CondExp pure_exp pure_exp pure_exp
+  | CondExp pure_exp pure_exp pure_exp (*TODO, not yet supported in Boogie formalization*)
   | FieldAcc pure_exp field_ident
-  | Old label pure_exp
+  | Old label pure_exp (*TODO*)
 
   | Perm pure_exp field_ident
-  | PermPred predicate_ident "pure_exp list"
+  | PermPred predicate_ident "pure_exp list" (*TODO*)
 
-  | FunApp function_ident "pure_exp list"
-  | Result (* Only for functions *)
+  | FunApp function_ident "pure_exp list" 
+  | Result (* Only for functions *) (*TODO*)
 
-\<comment>\<open>unfolding P(l) in e\<close>
-  | Unfolding predicate_ident "pure_exp list" pure_exp
+  | Unfolding predicate_ident "pure_exp list" pure_exp (*TODO*)
 
-  | Let pure_exp pure_exp
-  | PExists vtyp pure_exp
-  | is_pforall: PForall vtyp pure_exp
+  | Let pure_exp pure_exp (*TODO*)
+  | PExists vtyp pure_exp (*TODO*)
+  | is_pforall: PForall vtyp pure_exp (*TODO*)
 *)
 
-inductive syn_exp_rel :: "tr_vpr_bpl \<Rightarrow> viper_expr \<Rightarrow> boogie_expr \<Rightarrow> bool"
-  for Tr :: tr_vpr_bpl
+inductive syn_exp_rel :: "ViperLang.program \<Rightarrow> tr_vpr_bpl \<Rightarrow> viper_expr \<Rightarrow> boogie_expr \<Rightarrow> bool"
+  for Pr :: ViperLang.program and Tr :: tr_vpr_bpl
   where
     \<comment>\<open>The only global variables in the Boogie encoding are Heap and Mask, which do not have a variable 
        counter part in Viper.\<close>
        VarRel: 
        "\<lbrakk> var_translation Tr x = Some y \<rbrakk> \<Longrightarrow>
-          syn_exp_rel Tr (ViperLang.Var x) (Lang.Var y)"
+          syn_exp_rel Pr Tr (ViperLang.Var x) (Lang.Var y)"
      | LitRel: 
        "\<lbrakk> lit_translation Tr lit = e_bpl \<rbrakk> \<Longrightarrow>
-          syn_exp_rel Tr (ViperLang.ELit lit) e_bpl"
+          syn_exp_rel Pr Tr (ViperLang.ELit lit) e_bpl"
      | FieldAccRel:
-       "\<lbrakk> e_bpl = heap_read Tr (Lang.Var (heap_var Tr)) rcv_bpl f_bpl \<rbrakk> \<Longrightarrow>
-         syn_exp_rel Tr (FieldAcc e f) e_bpl"
+       "\<lbrakk> e_bpl = heap_read Tr (Lang.Var (heap_var Tr)) e_rcv_bpl e_f_bpl; 
+          syn_exp_rel Pr Tr e e_rcv_bpl;
+          (field_translation Tr f) = Some f_tr;
+          e_f_bpl = Lang.Var f_tr;
+          declared_fields Pr f \<noteq> None \<rbrakk> \<Longrightarrow>
+         syn_exp_rel Pr Tr (FieldAcc e f) e_bpl" \<comment>\<open>maybe \<^term>\<open>declared_fields Pr f \<noteq> None\<close> should be handled via \<^const>\<open>wf_pure_exp\<close> \<close>
      | UnopRel:
-       "\<lbrakk> unop_rel uop = uopb; syn_exp_rel Tr e e_bpl \<rbrakk> \<Longrightarrow>
-           syn_exp_rel Tr (ViperLang.Unop uop e) (Lang.UnOp uopb e_bpl)"
+       "\<lbrakk> unop_rel uop = uopb; 
+          syn_exp_rel Pr Tr e e_bpl \<rbrakk> \<Longrightarrow>
+          syn_exp_rel Pr Tr (ViperLang.Unop uop e) (Lang.UnOp uopb e_bpl)"
      | BinopRel:
-        "\<lbrakk> binop_rel bop = bopb; syn_exp_rel Tr e1 e1_bpl; syn_exp_rel Tr e2 e2_bpl \<rbrakk> \<Longrightarrow>
-           syn_exp_rel Tr (ViperLang.Binop e1 bop e2) (Lang.BinOp e1_bpl bopb e2_bpl)"
-     | FieldRel:
-        "syn_exp_rel Tr (Perm e f) e_bpl"
-     | FunAppRel:
+        "\<lbrakk> binop_rel bop = bopb;
+           bop \<noteq> IntDiv \<and> bop \<noteq> ViperLang.Mod; 
+           syn_exp_rel Pr Tr e1 e1_bpl; 
+           syn_exp_rel Pr Tr e2 e2_bpl \<rbrakk> \<Longrightarrow>
+           syn_exp_rel Pr Tr (ViperLang.Binop e1 bop e2) (Lang.BinOp e1_bpl bopb e2_bpl)"
+     | PermRel:
+         "\<lbrakk> e_bpl = mask_read Tr (Lang.Var (mask_var Tr)) rcv_bpl f_bpl; 
+           syn_exp_rel Pr Tr e rcv_bpl;
+           (field_translation Tr f) = Some f_tr;
+           f_bpl = Lang.Var f_tr;
+           declared_fields Pr f \<noteq> None \<rbrakk> \<Longrightarrow>
+           syn_exp_rel Pr Tr (Perm e f) e_bpl" \<comment>\<open>maybe \<^term>\<open>declared_fields Pr f \<noteq> None\<close> should be handled via \<^const>\<open>wf_pure_exp\<close> \<close>
+     | FunAppRel: \<comment>\<open>maybe should abstract over how function calls are encoded\<close>
        "\<lbrakk> es_bpl = e_heap#e_args_bpl; 
-          list_all2 (\<lambda>e_vpr e_bpl. syn_exp_rel Tr e_vpr e_bpl) es e_args_bpl;
+          fun_translation Tr f = Some f_bpl;
+          list_all2 (\<lambda>e_vpr e_bpl. syn_exp_rel Pr Tr e_vpr e_bpl) es e_args_bpl;          
           e_heap = Lang.Var (heap_var Tr) \<rbrakk> \<Longrightarrow>
-          syn_exp_rel Tr (FunApp f es) (FunExp f_bpl ts es_bpl)"
+          syn_exp_rel Pr Tr (FunApp f es) (FunExp f_bpl [] es_bpl)"
+
+lemma var_context_aux:
+  assumes "x \<in> set (map fst (snd \<Lambda>))"
+  shows "lookup_var \<Lambda> ns x = local_state ns x"
+proof -
+  from assms obtain y where "map_of (snd \<Lambda>) x = Some y"
+    by (metis domIff dom_map_of_2 not_Some_eq)
+  thus ?thesis
+    unfolding lookup_var_def
+    by simp
+qed
+
+definition lit_translation_rel :: "'a context_bpl => ('a vbpl_absval) nstate \<Rightarrow> (ViperLang.lit \<Rightarrow> Lang.expr) \<Rightarrow> bool"
+  where "lit_translation_rel ctxt ns litT \<equiv> (\<forall>lit e. litT lit = e \<longrightarrow> red_expr_bpl ctxt e ns (val_rel_vpr_bpl (val_of_lit lit)))"
+
+definition heap_read_wf :: "'a context_bpl \<Rightarrow> (boogie_expr \<Rightarrow> boogie_expr \<Rightarrow> boogie_expr \<Rightarrow> boogie_expr) \<Rightarrow> bool"
+  where 
+    "heap_read_wf ctxt hread \<equiv> \<forall> e_heap e_rcv e_f h r f ns v. 
+         ( (red_expr_bpl ctxt e_heap ns (AbsV (AHeap h)) \<and> 
+          red_expr_bpl ctxt e_rcv ns (AbsV (ARef r)) \<and>
+          red_expr_bpl ctxt e_f ns (AbsV (AField f)) \<and> h r f = Some v) \<longrightarrow>
+            red_expr_bpl ctxt (hread e_heap e_rcv e_f) ns v ) \<and>
+         ( (\<exists>v. red_expr_bpl ctxt (hread e_heap e_rcv e_f) ns v) \<longrightarrow>
+             (\<exists>v. red_expr_bpl ctxt e_rcv ns v) \<and> (\<exists>v. red_expr_bpl ctxt e_f ns v) )"
+
+definition mask_read_wf :: "'a context_bpl \<Rightarrow> (boogie_expr \<Rightarrow> boogie_expr \<Rightarrow> boogie_expr \<Rightarrow> boogie_expr) \<Rightarrow> bool"
+  where 
+    "mask_read_wf ctxt mread \<equiv> \<forall> e_mask e_rcv e_f m r f ns v. 
+         ( (red_expr_bpl ctxt e_mask ns (AbsV (AMask m)) \<and> 
+          red_expr_bpl ctxt e_rcv ns (AbsV (ARef r)) \<and>
+          red_expr_bpl ctxt e_f ns (AbsV (AField f)) \<and> m r f = v) \<longrightarrow>
+            red_expr_bpl ctxt (mread e_mask e_rcv e_f) ns (RealV v) ) \<and>
+         ( (\<exists>v. red_expr_bpl ctxt (mread e_mask e_rcv e_f) ns v) \<longrightarrow>
+             (\<exists>v. red_expr_bpl ctxt e_rcv ns v) \<and> (\<exists>v. red_expr_bpl ctxt e_f ns v) )"
+
+
+lemma bg_expr_list_red_iff:
+\<comment>\<open>Taken from Benjamin's BoogieWrapper.thy: TODO proper merge\<close>
+  "(A,\<Lambda>,\<Gamma>,\<Omega> \<turnstile> \<langle>[], s\<rangle> [\<Down>] v) = (v = [])"
+  "(A,\<Lambda>,\<Gamma>,\<Omega> \<turnstile> \<langle>e0#es, s\<rangle> [\<Down>] v)
+    = (\<exists>v0 vs. v = v0#vs \<and> (A,\<Lambda>,\<Gamma>,\<Omega> \<turnstile> \<langle>e0, s\<rangle> \<Down> v0) \<and> (A,\<Lambda>,\<Gamma>,\<Omega> \<turnstile> \<langle>es, s\<rangle> [\<Down>] vs))"
+  by ((rule iffI, (erule red_exprs.cases, assumption, simp), (simp, rule RedExpListNil)),
+      (rule iffI, (erule red_exprs.cases, simp, simp), (clarsimp, rule RedExpListCons; simp)))
+
+lemma bg_expr_list_red_all2:
+\<comment>\<open>Taken from Benjamin's BoogieWrapper.thy: TODO proper merge\<close>
+  "(A,\<Lambda>,\<Gamma>,\<Omega> \<turnstile> \<langle>es, s\<rangle> [\<Down>] vs) = list_all2 (\<lambda>e v. A,\<Lambda>,\<Gamma>,\<Omega> \<turnstile> \<langle>e, s\<rangle> \<Down> v) es vs"
+  by (induct es arbitrary:vs; simp add:bg_expr_list_red_iff list_all2_Cons1)
+
+lemma heap_read_wf_apply:
+  assumes "heap_read_wf ctxt hread" and
+          "h r f = Some v" and
+          "red_expr_bpl ctxt e_heap ns (AbsV (AHeap h))"and 
+          "red_expr_bpl ctxt e_rcv ns (AbsV (ARef r))" and
+          "red_expr_bpl ctxt e_f ns (AbsV (AField f))"
+  shows "red_expr_bpl ctxt (hread e_heap e_rcv e_f) ns v"
+  using assms
+  unfolding heap_read_wf_def
+  by blast
+
+lemma syn_exp_rel_correct:
+  assumes 
+          "syn_exp_rel Pr Tr e_vpr e_bpl" and 
+          "Pr, \<Delta>, None \<turnstile> \<langle>e_vpr; \<omega>\<rangle> [\<Down>]\<^sub>t Val v1" and
+
+         \<comment>\<open>Need Boogie expression to reduce because Viper has lazy binary operators but Boogie does not.
+           Thus, the Viper reduction on its own cannot be used to construct a Boogie reduction.\<close>
+          "\<exists>v. red_expr_bpl (create_ctxt_bpl A \<Lambda> \<Gamma>) e_bpl ns v" and
+
+          StateRel:"state_rel_vpr_bpl Pr \<Lambda> Tr \<omega> ns" and 
+          FInterpRel: "fun_interp_rel Pr (field_translation Tr) (fun_translation Tr) \<Delta> \<Gamma>" and
+          LitTrRel:"lit_translation_rel (create_ctxt_bpl A \<Lambda> \<Gamma>) ns (lit_translation Tr)"  and
+          HeapReadWf: "heap_read_wf (create_ctxt_bpl A \<Lambda> \<Gamma>) (heap_read Tr)" and
+          MaskReadWf: "mask_read_wf (create_ctxt_bpl A \<Lambda> \<Gamma>) (mask_read Tr)"
+        shows "red_expr_bpl (create_ctxt_bpl A \<Lambda> \<Gamma>) e_bpl ns (val_rel_vpr_bpl v1)"
+  using assms(1-3)
+proof(induction arbitrary: v1)
+  case (VarRel x y)
+  hence "get_store_total \<omega> x = Some v1"
+    by (auto elim: TotalExpressions.RedVar_case)
+  with StateRel \<open>var_translation Tr x = Some y\<close> show ?case
+    unfolding state_rel_vpr_bpl_def
+    by (metis context_bpl.select_convs(2) option.inject red_expr_red_exprs.RedVar)
+next
+  case (LitRel lit e_bpl)
+  hence "v1 = val_of_lit lit"
+    by (auto elim: TotalExpressions.RedLit_case)
+  hence "red_expr_bpl (create_ctxt_bpl A \<Lambda> \<Gamma>) e_bpl ns (val_rel_vpr_bpl v1)"
+    using LitRel LitTrRel
+    unfolding lit_translation_rel_def
+    by auto
+  thus ?case by simp
+next
+  case (FieldAccRel e_bpl e_rcv_bpl e_f_bpl e f f_tr)
+  from FieldAccRel.prems obtain a where "Pr, \<Delta>, None \<turnstile> \<langle>e;\<omega>\<rangle> [\<Down>]\<^sub>t Val (VRef (Address a))" and HeapVal:"get_hh_total_full \<omega> (a,f) = v1" 
+    using RedFieldNormal_case
+    by blast
+  hence LookupRcv:"A,\<Lambda>,\<Gamma>,[] \<turnstile> \<langle>e_rcv_bpl,ns\<rangle> \<Down> AbsV (ARef (Address a))"
+    using FieldAccRel.IH FieldAccRel.prems \<open>e_bpl = _\<close> HeapReadWf
+    unfolding heap_read_wf_def
+    by (metis context_bpl.select_convs(1) context_bpl.select_convs(2) context_bpl.select_convs(3) val_rel_vpr_bpl.simps(3))    
+  from \<open>declared_fields Pr f \<noteq> None\<close> StateRel obtain vty where 
+      FieldTy:"declared_fields Pr f = Some vty" and
+      LookupField:"lookup_var \<Lambda> ns f_tr = Some (AbsV (AField (NormalField f_tr vty)))"
+    unfolding state_rel_vpr_bpl_def
+    using FieldAccRel.hyps(3) by fastforce
+  from StateRel obtain h_bpl where
+     LookupHeap:"lookup_var \<Lambda> ns (heap_var Tr) = Some (AbsV (AHeap h_bpl))" and 
+     HeapRel:"heap_rel Pr (field_translation Tr) (get_hh_total_full \<omega>) h_bpl"
+    unfolding state_rel_vpr_bpl_def
+    by blast  
+  from HeapRel have
+    "has_Some ((=) (val_rel_vpr_bpl (get_hh_total_full \<omega> (a,f))))
+            (h_bpl (Address a) (NormalField f_tr vty))"
+    unfolding heap_rel_def
+    using FieldTy \<open>field_translation Tr f = Some f_tr\<close>
+    by (metis option.pred_inject(2) option.sel fst_conv snd_conv)
+  hence HeapValBpl:"h_bpl (Address a) (NormalField f_tr vty) = Some (val_rel_vpr_bpl v1)"
+    using HeapVal
+    by (metis (full_types) has_Some_iff)
+  show ?case 
+    apply (subst \<open>e_bpl =_ \<close>)
+    apply (rule heap_read_wf_apply[OF HeapReadWf])
+       apply (rule HeapValBpl)
+    by (auto intro: LookupHeap LookupRcv LookupField RedVar simp: \<open>e_f_bpl = expr.Var f_tr\<close>)
+next
+  case (UnopRel uop uopb e e_bpl)  
+  then show ?case 
+    by (auto elim!: TotalExpressions.RedUnop_case intro: Semantics.RedUnOp unop_rel_correct)
+next
+  case (BinopRel bop bopb e1 e1_bpl e2 e2_bpl)
+  from this obtain w2 where 
+        Red1:"\<exists>a. red_expr_bpl (create_ctxt_bpl A \<Lambda> \<Gamma>) e1_bpl ns a" and 
+        Red2:"red_expr_bpl (create_ctxt_bpl A \<Lambda> \<Gamma>) e2_bpl ns w2"
+    by auto
+  show ?case    
+  proof (rule RedBinop_case[OF \<open>Pr, \<Delta>, None \<turnstile> \<langle>Binop e1 bop e2; _\<rangle> [\<Down>]\<^sub>t _\<close>])    
+    \<comment>\<open>lazy binop case\<close>
+    fix v1'
+    assume a:"Pr, \<Delta>, None \<turnstile> \<langle>e1;\<omega>\<rangle> [\<Down>]\<^sub>t Val v1'" and eval_lazy:"eval_binop_lazy v1' bop = Some v1"
+    hence Red3:"red_expr_bpl (create_ctxt_bpl A \<Lambda> \<Gamma>) e1_bpl ns (val_rel_vpr_bpl v1')"
+      using BinopRel.IH(1) Red1
+      by auto
+    thus ?thesis
+      using binop_lazy_rel_correct[OF eval_lazy \<open>binop_rel _ = _\<close>] Red2
+      by (metis (no_types, hide_lams) BinopRel.prems(2) RedBinOp_case expr_eval_determ(1) option.distinct(1) option.sel)
+  next    
+    \<comment>\<open>nonlazy binop case\<close>
+    fix v1' v2'
+    assume "Pr, \<Delta>, None \<turnstile> \<langle>e1;\<omega>\<rangle> [\<Down>]\<^sub>t Val v1'" and 
+           "Pr, \<Delta>, None \<turnstile> \<langle>e2;\<omega>\<rangle> [\<Down>]\<^sub>t Val v2'" and 
+           "eval_binop v1' bop v2' = BinopNormal v1"
+    thus ?thesis
+      using BinopRel.IH Red1 Red2 \<open>binop_rel _ = _\<close> \<open>bop \<noteq> IntDiv \<and> bop \<noteq> ViperLang.binop.Mod\<close> binop_nonlazy_rel_correct      
+      by (blast intro: RedBinOp)
+  qed
+next
+  case (PermRel e_bpl e_rcv_bpl f_bpl e f f_tr)
+  from PermRel.prems obtain r where "Pr, \<Delta>, None \<turnstile> \<langle>e;\<omega>\<rangle> [\<Down>]\<^sub>t Val (VRef r)" 
+    using RedPerm_case
+    by blast  
+
+  from \<open>declared_fields Pr f \<noteq> None\<close> StateRel obtain vty where 
+      FieldTy:"declared_fields Pr f = Some vty" and
+      LookupField:"lookup_var \<Lambda> ns f_tr = Some (AbsV (AField (NormalField f_tr vty)))"
+    unfolding state_rel_vpr_bpl_def
+    using PermRel by fastforce
+  from StateRel obtain m_bpl where
+     LookupMask:"lookup_var \<Lambda> ns (mask_var Tr) = Some (AbsV (AMask m_bpl))" and 
+     MaskRel:"mask_rel Pr (field_translation Tr) (get_mh_total_full \<omega>) m_bpl"
+    unfolding state_rel_vpr_bpl_def
+    by blast
+
+  show ?case
+  proof (rule RedPerm_case)
+    show "Pr, \<Delta>, None \<turnstile> \<langle>Perm e f;\<omega>\<rangle> [\<Down>]\<^sub>t Val v1"
+      by (auto intro: PermRel)
+  next
+    assume "v1 = VPerm 0"
+    assume "Pr, \<Delta>, None \<turnstile> \<langle>e;\<omega>\<rangle> [\<Down>]\<^sub>t Val (VRef Null)"
+    hence "A,\<Lambda>,\<Gamma>,[] \<turnstile> \<langle>e_rcv_bpl,ns\<rangle> \<Down> AbsV (ARef Null)"
+      using PermRel.IH PermRel.prems \<open>e_bpl = _\<close> MaskReadWf
+      unfolding mask_read_wf_def
+      by (metis context_bpl.select_convs(1) context_bpl.select_convs(2) context_bpl.select_convs(3) val_rel_vpr_bpl.simps(3))
+    with LookupField LookupMask MaskRel MaskReadWf \<open>e_bpl = _\<close> PermRel.hyps \<open>v1 = _\<close>
+    show ?case
+      unfolding mask_rel_def mask_read_wf_def
+      by (metis context_bpl.select_convs(1) context_bpl.select_convs(2) context_bpl.select_convs(3) of_rat_0 red_expr_red_exprs.RedVar val_rel_vpr_bpl.simps(5))
+  next
+    fix a
+    assume "v1 = VPerm (Rep_prat (fst (snd (Rep_total_state (snd (snd \<omega>)))) (a, f)))"
+    hence HeapVal:"v1 = VPerm (Rep_prat (get_mh_total_full \<omega> (a,f)))"
+      by simp
+    assume "Pr, \<Delta>, None \<turnstile> \<langle>e;\<omega>\<rangle> [\<Down>]\<^sub>t Val (VRef (Address a))"
+    hence "A,\<Lambda>,\<Gamma>,[] \<turnstile> \<langle>e_rcv_bpl,ns\<rangle> \<Down> AbsV (ARef (Address a))"
+      using PermRel.IH PermRel.prems \<open>e_bpl = _\<close> MaskReadWf
+      unfolding mask_read_wf_def
+      by (metis context_bpl.select_convs(1) context_bpl.select_convs(2) context_bpl.select_convs(3) val_rel_vpr_bpl.simps(3))
+
+    with LookupMask LookupField MaskReadWf \<open>e_bpl = _\<close> MaskRel
+    show ?case
+      unfolding mask_read_wf_def mask_rel_def
+      by (simp add: FieldTy HeapVal PermRel.hyps(3) PermRel.hyps(4) if_Some_iff red_expr_red_exprs.RedVar)
+  qed
+next
+  case (FunAppRel es_bpl e_heap e_args_bpl f f_bpl es)
+  from \<open>Pr, \<Delta>, None \<turnstile> \<langle>FunApp f es;\<omega>\<rangle> [\<Down>]\<^sub>t Val v1\<close>
+  obtain vs f_interp_vpr where     
+      args_vpr: "list_all2 (\<lambda>e v. red_pure_exp_total Pr \<Delta> None e \<omega> (Val v)) es vs" and
+                "\<Delta> f = Some f_interp_vpr" and
+                "f_interp_vpr vs \<omega> = Some (Val v1)"
+    by (blast elim: red_pure_exp_total_elims)
+ 
+  from this obtain vs_bpl where BplArgsRed:"list_all2 (\<lambda>e v. red_expr A \<Lambda> \<Gamma> [] e ns v) es_bpl vs_bpl"
+    using \<open>\<exists>a. red_expr_bpl (create_ctxt_bpl A \<Lambda> \<Gamma>) (FunExp f_bpl [] es_bpl) ns a\<close>    
+    by (auto simp: bg_expr_list_red_all2)
+  have "length es = length e_args_bpl" using FunAppRel.IH
+    by (simp add: List.list_all2_conv_all_nth)
+ have "length es = length vs" using args_vpr
+      by (simp add: List.list_all2_conv_all_nth)
+
+  have "list_all2 (\<lambda>e v. red_expr A \<Lambda> \<Gamma> [] e ns (val_rel_vpr_bpl v)) e_args_bpl vs"  
+  proof (rule List.list_all2_all_nthI)
+    show "length e_args_bpl = length vs"
+      using \<open>length es = length e_args_bpl\<close> \<open>length es = length vs\<close>
+      by simp
+  next
+    fix n
+    assume "n < length e_args_bpl"
+    hence "n < length es" using \<open>length es = length e_args_bpl\<close>
+      by simp
+
+    hence IHReq1:"Pr, \<Delta>, None \<turnstile> \<langle>es ! n;\<omega>\<rangle> [\<Down>]\<^sub>t Val (vs ! n)"
+      using args_vpr
+      by (metis list_all2_conv_all_nth)
+
+    have "red_expr_bpl (create_ctxt_bpl A \<Lambda> \<Gamma>) (es_bpl ! (Suc n)) ns (vs_bpl ! (Suc n))"
+      using BplArgsRed \<open>n < length e_args_bpl\<close>    
+      by (auto simp: \<open>es_bpl = _\<close> list_all2_conv_all_nth)
+    hence IHReq2: "\<exists>v. red_expr_bpl (create_ctxt_bpl A \<Lambda> \<Gamma>) (e_args_bpl ! n) ns v"
+      by (auto simp: \<open>es_bpl = _\<close>)
+
+    from IHReq1 IHReq2 FunAppRel.IH      
+    show "A,\<Lambda>,\<Gamma>,[] \<turnstile> \<langle>e_args_bpl ! n,ns\<rangle> \<Down> val_rel_vpr_bpl (vs ! n)"
+      by (auto simp: \<open>n < length e_args_bpl\<close> list_all2_conv_all_nth)
+  qed      
+
+  hence *:"list_all2 (\<lambda>e v. red_expr A \<Lambda> \<Gamma> [] e ns v) e_args_bpl (map val_rel_vpr_bpl vs)"
+    by (simp add: list.rel_map(2))
+
+  from StateRel obtain h_bpl where
+     LookupHeap:"lookup_var \<Lambda> ns (heap_var Tr) = Some (AbsV (AHeap h_bpl))" and 
+     HeapRel:"heap_rel Pr (field_translation Tr) (get_hh_total_full \<omega>) h_bpl"
+    unfolding state_rel_vpr_bpl_def
+    by blast
+
+  from LookupHeap have "red_expr_bpl (create_ctxt_bpl A \<Lambda> \<Gamma>) (Var (heap_var Tr)) ns (AbsV (AHeap h_bpl))"
+    by (auto intro: Semantics.RedVar)
+  with * have A:"list_all2 (\<lambda>e v. red_expr A \<Lambda> \<Gamma> [] e ns v) ((Var (heap_var Tr))#e_args_bpl) ((AbsV (AHeap h_bpl))#(map val_rel_vpr_bpl vs))"
+    by simp
+
+  obtain f_interp_bpl where
+       "\<Gamma> f_bpl = Some f_interp_bpl" and
+       "fun_rel Pr (field_translation Tr) f_interp_vpr f_interp_bpl"
+    using FInterpRel \<open>fun_translation Tr f = Some f_bpl\<close> \<open>\<Delta> f = Some f_interp_vpr\<close>
+    unfolding fun_interp_rel_def
+    by (metis has_Some_iff)
+
+  hence **:"(eval_heap_dep_bpl_fun f_interp_bpl (map val_rel_vpr_bpl vs) (AbsV (AHeap h_bpl))) = Some (val_rel_vpr_bpl v1)"
+    using \<open>f_interp_vpr vs \<omega> = Some (Val v1)\<close> HeapRel
+    unfolding fun_rel_def 
+    apply (simp add: has_Some_iff)
+    by (metis prod.collapse)    
+  show ?case
+    apply (rule RedFunOp)
+      apply (simp add: \<open>\<Gamma> f_bpl = Some f_interp_bpl\<close>)     
+     apply (simp add: bg_expr_list_red_all2)
+     apply (subst \<open>es_bpl = _\<close>)
+    apply (subst \<open>e_heap = _\<close>)    
+     apply (rule A)
+    using **
+    by simp
+qed
+
 
 end
